---
title: "Assignment 2"
author: "Simon"
date: "7/10/2021"
output: 
  bookdown::pdf_document2: default
---

# Endogenous growth theory:

Assume production function of final goods sector is given by:

```{=tex}
\begin{equation}
Y(t) = [(1-\alpha_K) K(t)\alpha][A(t)(1-\alpha_L)L(t)]^{1-\alpha} (\#eq:prod_f)
\end{equation}
```

where $1- \alpha_L$ and $1- \alpha_K$ is the proportion of labour and capital allocated for final production.

**Capital stock** is given by:

```{=tex}
\begin{equation}
\dot K(t) = sY(t) (\#eq:K_f)
\end{equation}
```

**Production function** of R&D sector is given by:

```{=tex}
\begin{equation}
\dot A(t) = B[\alpha_K K(t)]^\beta [\alpha_L L(t)]^\gamma A(t)^\theta (\#eq:A_f)
\end{equation}
```



**Population growth** is exogenous:

$$\dot L(t) = nL(t)$$

## Derive an expression for the growth rate of capital gK(t) and growth rate of technology gA(t)

**Growth rate of Capital**

We start by substituteing \@ref(eq:prod_f) into equation \@ref(eq:K_f):

$$\dot K(t) = s(1-\alpha)^\alpha (1- \alpha _L )^{1-\alpha} K(t)^\alpha A(t)^{1- \alpha} L_(t)^{1-\alpha}$$
we can write $c_K=  s(1-\alpha)^\alpha (1- \alpha _L )^{1-\alpha}$

So we get: 

$$\dot K(t) = C_K K(t)^\alpha A(t)^{1- \alpha} L(t)^{1-\alpha}$$
We divide the expresion by $K(t)$ so we can write $\alpha - 1$ in the exponent. 

$$\frac {\dot K(t)}{K(t)} = C_K K(t)^{\alpha- 1} A(t)^{1- \alpha} L(t)^{1-\alpha}$$
We can now chance $K(t)^{\alpha - 1}$ changing the sign of the exponent so $\frac{1}{K(t)^{1 - \alpha}}$ We can then set $1- \alpha$ out as a common exponent. 


$$\frac {\dot K(t)}{k(t)} = C_K [\frac{A(t) L(t)}{K(t)}]^{1-\alpha}$$


**Growth rate of technology**

We divide equation \@ref(eq:A_f) by $A(t)$: 


$$\frac{\dot A(t)}{A(t)} = B[\alpha_K K(t)]^\beta [\alpha_L L(t)]^\gamma A(t)^{\theta-1}$$
For simplicity we can write the constant $B\alpha^\beta _K \alpha^\gamma _L$ as equal to $C_\alpha$.


$$\frac{\dot A(t)}{A(t)} = C_\alpha K(t)^\beta L(t)^\gamma A(t)^{\theta-1}$$

## Spg 2


We start with the expression from the previous question $g_A(t)= C_\alpha K(t)^\beta L(t)^\gamma A(t)^{\theta-1}$

We now take the log and differentiate by time: 

$$\frac{\dot g_A(t)}{g_A(t)}= \beta g_K(t) + \gamma n + (\theta - 1) g_A(t)$$
We can set this equation equal to 0 as we know $\frac{\dot g_A(t)}{g_A(t)}=0$ in steady state.

$$\beta g_K^*(t) + \gamma n + (\theta - 1) g_A^*(t)=0$$

As we know both $g_K(t)$ and $g_A(t)$ are equal to 0 in steady state we can look at equation $\frac{\dot {g_K}}{g_K}= (1- \alpha) [g_A + n - g_K]$ And see that when $\frac{\dot {g_K}}{g_K}$ and we are in steady state this can also be written as: 

$$g^*_A +n -g^*_K=0$$
This can be re-written: 


$$g^*_A +n =g^*_K$$
We can now substitute this into the equation: 

$$\beta (g^*_A +n)  + \gamma n + (\theta - 1) g^*_A=0$$
We want to move all terms not including $g_A^*$ to the right site.

$$\beta g^*_A+ (1-\theta)g^*_A= -(\beta + \gamma)n$$
We move $g_A^*$ out as a common factor.

$$g_A^*(\beta + (\theta - 1))= -(\beta + \gamma)n$$
we change the sign on both sites. 

$$g_A^*(1 - (\theta + \beta))= (\beta + \gamma)n$$
And last we divide by $(1 - (\theta + \beta))$

$$g_A^*= \frac{(\beta + \gamma)}{(1 - (\theta + \beta))}n$$
- We can see the growth rate of technology in steady state is effected by $\beta$ (elasticity of capital on knowledge??????). 
- $\gamma$ is the output elasticity of labour allocated in R&D which we can see has a positive effect on the growth rate.
- $\theta$ is a parameter describing the elasticity of existing knowledge (A), we can see this also has a positive effect on $g^*_A$





# Real business cycle theory

Assume the following utility function:


$$u_t= ln[c_t] + \frac{b(1-l_t)^{1-\gamma}}{1-\gamma}$$
where, $c_t$ is consumption, $b > 0$, and $\gamma > 0$

Income of the individual is equal to $w_tl_t$

where, $w_t$ is wage, and $l_t$ is the labour supply

## Define the budget constraint and answer the following:

First I define the budget constraint:

$$C=wl$$

**How, if at all, does labour supply depend on wage?**

We can now set up the langrange 

$$L= ln[C_t]+ \frac{b(1-l_t)^{1-\gamma}}{1-\gamma} + \lambda (wl-C_t)$$
We now differntiate with respect to $C_t$ and $l_t$

$$\frac {\delta L}{\delta C_t}= \frac{1}{C_t} - \lambda =0$$
$$\frac {\delta L}{\delta l_t}= -b(1-l_t)^{-\gamma}+ w\lambda=0$$

The first equation $\frac{1}{C_t} - \lambda$ we can re-write using the budget constraint $C=wl$ or $\frac{1}{C_t} = \frac{1}{wl}$ we can therfore write:

$$\frac{1}{wl}=\lambda$$
We can now substitute thes into the second equation $-b(1-l_t)^{-\gamma}+ w\lambda=0$: 

$$-b(1-l_t)^{-\gamma}= \frac{1}{l_t}$$
Allready now we can see that $w$ is no longer in the equation so it would have no effect on labour supply. 



**Explain why!!!**



## Re-consider the above problem for two periods: 

$$u= ln[C_1] + \frac{b(1-l_1)^{1-\gamma}}{1-\gamma} + e^{- \rho} [ln[C_2] + \frac{b(1-l_2)^{1-\gamma}}{1-\gamma}]$$
where 

- Periode 1 consumption $C_1 = w_1l_1$
- Periode 2 consumption $C_2 = w_2l_2 + s_1(1+r)$ where $s_1= w_1l_1 - C_1$. 

## Define the budget constraint and give intuitive answers to the following questions after solving the problem:

To get the budget constraint we first re-write $C_2$: 

$$C_2 = w_2l_2 +  (w_1l_1 - C_1)(1+r)$$
We divide by $(1+r)$ and isolate the consumption for periode 1 and 2 on the left site. 

$$C_1+ \frac{C_2}{(1+r)} = w_1 l_1 + w_2 l_2* \frac{1}{(1+r)}$$

We now have the budget constraint, and we can set up the langrange equation. 

$$L= ln[C_1] + \frac{b(1-l_1)^{1-\gamma}}{1-\gamma} + e^{- \rho} [ln[C_2] + \frac{b(1-l_2)^{1-\gamma}}{1-\gamma}] + \lambda [w_1l_1 + w_2l_2 * \frac{1}{(1+r)} - C_1 - \frac{C_2}{(1+r)}]$$
Now i differentiate with respcect to $l_1$ and $l_2$:

- For $l_1$

$$-b(1-l_1)^{-\gamma} +w_1 \lambda= 0$$

- For $l_2$

$$-e^{- \rho}b(1-l_2)^{- \gamma} + \frac {w_2 \lambda} {(1+r)}=0$$
We isolate lambda in the equation for $l_1$ and then substitute into the equation for $l_2$


$$-e^{- \rho}b(1-l_2)^{- \gamma}+ \frac {w_2 \frac{b(1-l_1)^{- \gamma}}{w_1}}{(1+r)} =0$$

We need to isolate so we get $\frac{(1-l_2)}{(1-l_1)}$ 

We can split up the fraction and collect the $w$ expressions in one fraction. 

$$-e^{- \rho}b(1-l_2)^{- \gamma}+ \frac {w_2}{(1+r)}* \frac{b(1-l_1)^{- \gamma}}{w_1} =0$$
Kan jeg godt gøre det? burde jeg ik vende brøkken om?


$$-e^{- \rho}b(1-l_2)^{- \gamma}+ \frac {w_2}{w_1}* \frac{b(1-l_1)^{- \gamma}}{(1+r)} =0$$
We can now divide with $b(1-l_1)^{- \gamma}$ 

$$-e^{- \rho} \frac{b(1-l_2)^{- \gamma}}{b(1-l_1)^{- \gamma}}+ \frac {w_2}{w_1}* \frac{1}{(1+r)} =0$$
We can now move the second term on the other site of the equal sign

$$-e^{- \rho} \frac{b(1-l_2)^{- \gamma}}{b(1-l_1)^{- \gamma}} =- \frac {w_2}{w_1}* \frac{1}{(1+r)}$$
We can remove the $- \gamma$ and $b$ so we end up with: 

$$-e^{- \rho} \frac{(1-l_2)}{(1-l_1)} =- \frac {w_2}{w_1}* \frac{1}{(1+r)}$$
We can now multiply with $\frac{1}{-e^-\rho}$

And we end up with the following equation:

$$\frac{(1-l_2)}{(1-l_1)} = \frac {w_2}{w_1}* \frac{1}{(1+r)e^{- \rho}}$$
We can take the inverse on both sites:

$$\frac{(1-l_1)}{(1-l_2)} = \frac {w_1}{w_2}* \frac{1}{(1+r)e^{- \rho}}$$

- How does the relative demand for leisure $\frac{(1-l_1)}{(1-l_2)}$ depend on the relative wage $\frac{w_1}{w_2}$. 

We can see that if the relative wage $\frac{w_1}{w_2}$ increases which means the wage in periode 1 is now higher relative to the one in periode 2. $\frac{(1-l_1)}{(1-l_2)}$ would also have to increase meaning $l_1$ needs to fall and/or $l_2$ needs to increase. 


- How does the relative demand for leisure $\frac{(1-l_1)}{(1-l_2)}$ depend on the interest rate (r)?

We can see if $r$ increases we get that the right hand site will decrease, this means $\frac{(1-l_1)}{(1-l_2)}$ also should decrease. For this to happen $l_1$ needs to increase, and/or $l_2$ needs to increase. makes since as a higher interres rate means i can work more in periode 1 to have more savings that increases my income. 








